execution/tests/BATTests/BATGens.v
@@ -1,0 +1,43 @@
+From ConCert Require Import Blockchain BAT.
+From ConCert Require Import Serializable.
+From ConCert Require Import Containers.
+From ConCert.Execution.QCTests Require Import TestUtils.
+
+From QuickChick Require Import QuickChick. Import QcNotation.
+From ExtLib.Structures Require Import Monads.
+Import MonadNotation. Open Scope monad_scope.
+From Coq Require Import List ZArith. Import ListNotations.
+
+Module Type BATGensInfo.
+  Parameter contract_addr : Address.
+  Parameter gAccount : Chain -> G Address.
+End BATGensInfo.
+
+Module BATGens (Info : BATGensInfo).
+Import Info.
+Arguments SerializedValue : clear implicits.
+Arguments deserialize : clear implicits.
+Arguments serialize : clear implicits.
+
+Definition serializeMsg := @serialize BAT.Msg _.
+
+(*
+  Generate create token requests on the form (from_addr, value, create_tokens)
+  Has chance to generate request from both existing and new accounts
+*)
+Definition gCreateTokens (state : BAT.State) : G (Address * Amount * Msg) :=
+  let nr_accounts_in_state := FMap.size (balances state) in
+  let weight_1 := nr_accounts_in_state in
+  let randomize_mk_gen g :=
+    freq [
+      (weight_1, returnGen g) ;
+      (0, from_addr <- arbitrary ;; returnGen (from_addr, choose (0,3), create_tokens))
+    ] in
+  sample <- sampleFMapOpt (balances state) ;;
+  match sample with
+  | Some (from_addr, _) => randomize_mk_gen (from_addr, choose(0,3), create_tokens)
+  | None => from_addr <- arbitrary ;; returnGen (from_addr, choose(0,3), create_tokens)
+  end.
+  
+
+
